Basic skeleton

TestModels/Streaming/src/SimpleStreamingImpl.dfy
@@ -3,6 +3,8 @@
 // Do not modify this file. This file is machine generated, and any changes to it will be overwritten.
 include "../Model/SimpleStreamingTypes.dfy"
 module SimpleStreamingImpl refines AbstractSimpleStreamingOperations {
+  import opened StandardLibrary.Actions
+
   datatype Config = Config
   type InternalConfig = Config
   predicate ValidInternalConfig?(config: InternalConfig)
@@ -12,13 +14,46 @@ module SimpleStreamingImpl refines AbstractSimpleStreamingOperations {
   predicate CountBitsEnsuresPublicly(input: CountBitsInput , output: Result<CountBitsOutput, Error>)
   {true}
 
+  class BitCounter extends Action<StreamEvent<seq<uint8>, Error>, ()> {
+
+    var sumSoFar: int32
+    const outStream: Stream<StreamEvent<int32, Error>>
+
+    constructor(outStream: Stream<StreamEvent<int32, Error>>) 
+      ensures fresh(Repr)
+    {
+      sumSoFar := 0;
+      this.outStream := outStream;
+      Repr := {};
+    }
+
+    method Call(value: StreamEvent<seq<uint8>, Error>) returns (nothing: ()) 
+      modifies Repr
+    {
+      assume this in Repr;
+      assume outStream.Repr <= Repr;
+      match value {
+        case Some(bits) => {
+          // TODO: actually count bits. Just guessing the average (like guessing all C's on a test :) 
+          assume sumSoFar < 10000;
+          sumSoFar := sumSoFar + 4;
+        }
+        case None => {
+          outStream.Put(Some(Success(sumSoFar)));
+        }
+      }
+      return ();
+    }
+  }
 
 
   method CountBits ( config: InternalConfig , input: CountBitsInput )
     returns (output: Result<CountBitsOutput, Error>)
-
   {
-    expect false, "...that you'll fill this in";
+    var outStream := new SimpleStream<StreamEvent<int32, Error>>();
+    var counter := new BitCounter(outStream);
+    input.bits.OnNext(counter);
+    return Success(CountBitsOutput(sum := outStream));
   }
 
 
@@ -31,7 +66,12 @@ module SimpleStreamingImpl refines AbstractSimpleStreamingOperations {
     returns (output: Result<BinaryOfOutput, Error>)
 
   {
-    expect false, "...that you'll fill this in";
+    // TODO: Actually compute the binary
+    var fakeBinary := [Success([12]), Success([34, 56])];
+    var fakeBinaryIter := new SeqEnumerator(fakeBinary);
+    var outStream := new LazyStream<Result<seq<uint8>, Error>>(fakeBinaryIter);
+
+    return Success(BinaryOfOutput(binary := outStream));
   }
 
 
@@ -39,11 +79,42 @@ module SimpleStreamingImpl refines AbstractSimpleStreamingOperations {
   {true}
 
 
+  class Chunker extends Action<StreamEvent<seq<uint8>, Error>, ()> {
+
+    const outStream: Stream<StreamEvent<seq<uint8>, Error>>
+
+    constructor(outStream: Stream<StreamEvent<seq<uint8>, Error>>)
+      ensures fresh(Repr) 
+    {
+      this.outStream := outStream;
+      Repr := {};
+    }
+
+    method Call(value: StreamEvent<seq<uint8>, Error>) returns (nothing: ()) 
+      modifies Repr
+    {
+      assume this in Repr;
+      assume outStream.Repr <= Repr;
+      match value {
+        case Some(bits) => {
+          outStream.Put(Some(bits));
+        }
+        case None => {
+          outStream.Put(None);
+        }
+      }
+      return ();
+    }
+  }
 
   method Chunks ( config: InternalConfig , input: ChunksInput )
     returns (output: Result<ChunksOutput, Error>)
 
   {
-    expect false, "...that you'll fill this in";
+    var outStream := new SimpleStream<StreamEvent<seq<uint8>, Error>>();
+    var chunker := new Chunker(outStream);
+    input.bytesIn.OnNext(chunker);
+
+    return Success(ChunksOutput(bytesOut := outStream));
   }
 }
