TestModels/dafny-dependencies/StandardLibrary/src/Actions.dfy
@@ -11,20 +11,21 @@ module StandardLibrary.Actions {
   // Then you have a history that ties the behavior
   // of the methods together,
   // supporting constraints on the order of calls etc.
-  trait Action<T, R> {
-    ghost var history: seq<(T, R)>
+  trait {:termination false} Action<T, R> {
+    // ghost var history: seq<(T, R)>
 
-    predicate Consumes(history: seq<(T, R)>, next: T)
-    predicate Produces(history: seq<(T, R)>)
-    
+    // predicate Consumes(history: seq<(T, R)>, next: T)
+    // predicate Produces(history: seq<(T, R)>)
+    var Repr: set<object>
 
     method Call(t: T) returns (r: R)
+      modifies Repr
       // requires Consumes(history, t)
 
   }
 
   // TODO: could use different words for calling when there is no input/no output
-  method Call<T>(a: Action<T, ()>, t: T) {
+  method Call<T>(a: Action<T, ()>, t: T) modifies a.Repr {
     var _ := a.Call(t);
   }
 
@@ -36,10 +37,123 @@ module StandardLibrary.Actions {
     | true 
     witness *
 
-  predicate ConsumesAnything<T(!new), R(!new)>(a: Action<T, R>) {
-    forall history, next | a.Produces(history) :: a.Consumes(history, next)
+  class SeqEnumerator<T> extends Action<(), Option<T>> {
+
+    var values: seq<T>
+
+    constructor(values: seq<T>) {
+      this.values := values;
+    }
+
+    method {:verify false} Call(input: ()) returns (value: Option<T>) 
+      modifies Repr
+    {
+      if |values| == 0 {
+        value := None;
+      } else {
+        value := Some(values[0]);
+        values := values[1..];
+      }
+    }
+
   }
 
-  // TODO: consumes any None-terminated sequence of inputs
-  predicate ConsumesTerminated<T(!new), R(!new)>(a: Action<Option<T>, R>)
+
+  // TODO: This is a finite stream really,
+  // ideally this would be a specific instance of an infinite stream
+  // of Option<T> just like Action<(), T>
+  // TODO: Do we need to signal back pressure or cancellation?
+  // Could return something from OnNext
+  trait Stream<T> {
+
+    var Repr: set<object>
+
+    method Put(t: T)
+      modifies Repr
+
+    method OnNext(a: Action<T, ()>)
+      modifies Repr, a.Repr
+
+  }
+
+  // Similar to Result, but for delivering a sequence of values instead of just one
+  type StreamEvent<T, E> = Option<Result<T, E>>
+
+  // Cheating for now, since this can't block
+  class SimpleStream<T(0)> extends Stream<T> {
+
+    var values: seq<T>
+    var callbacks: seq<Action<T, ()>>
+
+    constructor() {
+      values := [];
+    }
+
+    predicate Valid() 
+      reads this, Repr
+    {
+      && this in Repr
+      && forall a <- callbacks :: a in Repr && a.Repr <= Repr
+    }
+
+    method {:verify false} Put(value: T)
+      modifies Repr
+    {
+      values := values + [value];
+
+      for i := 0 to |callbacks| 
+        invariant callbacks == old(callbacks)
+      {
+        var callback := callbacks[i];
+        var _ := callback.Call(value);
+      }
+    }
+
+    method OnNext(a: Action<T, ()>)
+      modifies Repr
+    {
+      assume Valid();
+      callbacks := callbacks + [a];
+    }
+
+  }
+
+  class LazyStream<T(0)> extends Stream<Option<T>> {
+
+    const iter: Action<(), Option<T>>
+    var callbacks: seq<Action<Option<T>, ()>>
+
+    constructor(iter: Action<(), Option<T>>) {
+      this.iter := iter;
+    }
+
+    predicate Valid() 
+      reads this, Repr
+    {
+      && this in Repr
+      && iter in Repr && iter.Repr <= Repr
+      && forall a <- callbacks :: a in Repr && a.Repr <= Repr
+    }
+
+    method Put(value: Option<T>)
+      modifies Repr
+    {
+      expect false;
+    }
+
+    method {:verify false} OnNext(a: Action<Option<T>, ()>)
+      modifies Repr
+    {
+      // TODO: Actual Action specs to prove this terminates
+      while (true) {
+        var next := iter.Call(());
+        var _ := a.Call(next);
+
+        if next == None {
+          break;
+        }
+      }
+    }
+
+  }
 }
